theories/clang/lib/interrupt.v
@@ -3,7 +3,7 @@
 Require Import logic.
 
 Section definitions.
-  Context `{!clangG Σ} {invs: nat → iProp Σ}.
+  Context `{!clangG Σ} {invs: nat → iProp Σ} {ptot: nat}.
 
   Fixpoint INVS (p: nat) :=
     match p with
@@ -17,6 +17,13 @@ Section definitions.
       | S p' => INVS p'
     end.
 
+  Fixpoint INVS_range (p: nat) (q: nat) : iProp Σ :=
+    if bool_decide (p > q) then True%I
+    else match q with
+           | O => invs O
+           | S q' => (invs q ∗ INVS_range p q')%I
+         end.
+
   (* Interface *)
 
   Structure interrupt := Interrupt {
@@ -24,31 +31,40 @@ Section definitions.
     name : Type;
     f_sti: ident;
     f_cli: ident;
+    f_create_task: ident;
     hpri (γp: name) (i: nat) : iProp Σ;
     closed (γ: name): iProp Σ;
-    int_ctx (N: namespace) (γ γp: name): iProp Σ;
+    int_ctx (γ γp: name): iProp Σ;
     (* -- general properties -- *)
-    int_ctx_persistent N γ γp : PersistentP (int_ctx N γ γp);
+    int_ctx_persistent γ γp : PersistentP (int_ctx γ γp);
     closed_timeless γ : TimelessP (closed γ);
-    closed_exclusive γ : closed γ -∗ closed γ -∗ False;
+    closed_exclusive γ : closed γ -∗ closed γ -∗ False; (* can't close twice *)
     (* HACK *)
     sti : expr := Ecall f_sti [];
     cli : expr := Ecall f_cli [];
+    create_task (f: ident) (p: nat): expr := Ecall f_create_task [Eident f; Enat p];
     sti_nj: is_jmp sti = false;
     cli_nj: is_jmp cli = false;
     (* -- operation specs -- *)
-    sti_spec N prio γ γp Φ :
-      int_ctx N γ γp ∗ hpri γp prio ∗ INVS_up prio ∗ closed γ ∗ (hpri γp prio -∗ Φ Vvoid)
+    create_task_spec E f e prio Φ :
+      text_interp f (Function Tvoid [] e) ∗
+      (∀ N: namespace,
+         (|={⊤, ⊤∖↑N}=> INVS_range prio ptot) -∗
+         (INVS_range prio ptot ={⊤, ⊤∖↑N}=∗ True) -∗
+         WP e {{ v, True%I}})
+      ⊢ WP create_task f prio @ E {{ Φ }};
+    sti_spec prio γ γp Φ :
+      int_ctx γ γp ∗ hpri γp prio ∗ INVS_up prio ∗ closed γ ∗ (hpri γp prio -∗ Φ Vvoid)
       ⊢ WP sti {{ Φ }};
-    cli_spec N prio γ γp Φ :
-      int_ctx N γ γp ∗ hpri γp prio ∗ (INVS_up prio -∗ hpri γp prio -∗ closed γ -∗ Φ Vvoid)
+    cli_spec prio γ γp Φ :
+      int_ctx γ γp ∗ hpri γp prio ∗ (INVS_up prio -∗ hpri γp prio -∗ closed γ -∗ Φ Vvoid)
       ⊢ WP cli {{ Φ }}
   }.
 End definitions.
 
 Existing Instances int_ctx_persistent closed_timeless.
 
-Arguments interrupt {_ _} _.
-Arguments hpri {_ _} _ {_} _ _.
-Arguments closed {_ _} _ {_} _.
+Arguments interrupt {_ _} _ _.
+Arguments hpri {_ _} _ {_ _} _ _.
+Arguments closed {_ _} _ {_ _} _.
 Arguments int_ctx {_ _} _ {_} _ _ _.
